src/HaskProofToLatex.v
@@ -6,7 +6,6 @@ Generalizable All Variables.
 Require Import Preamble.
 Require Import General.
 Require Import NaturalDeduction.
-Require Import NaturalDeductionToLatex.
 Require Import Coq.Strings.String.
 Require Import Coq.Lists.List.
 Require Import HaskKinds.
