Makefile
@@ -1,4 +1,4 @@
-coqc     := coqc -noglob
+coqc     := coqc -noglob -opt
 coqfiles := $(shell find src -name \*.v  | grep -v \\\#)
 allfiles := $(coqfiles) $(shell find src -name \*.hs | grep -v \\\#)
 
@@ -6,7 +6,7 @@ default: build/CoqPass.hs
 
 build/CoqPass.hs: $(allfiles)
 	make build/Makefile.coq
-	cd build; make -f Makefile.coq OPT=-dont-load-proofs ExtractionMain.vo
+	cd build; make -f Makefile.coq OPT="-opt -dont-load-proofs" ExtractionMain.vo
 	cd build; make -f Makefile.coq Extraction.vo
 	cat src/Extraction-prefix.hs                                     > build/CoqPass.hs
 	cat build/Extraction.hs | grep -v '^module' | grep -v '^import' >> build/CoqPass.hs
